theories/CongLtLemma.v
@@ -3,75 +3,10 @@ Require Import ProcSyn.
 Require Import Semantics.
 Require Import unscoped.
 Require Import core.
+Require Import SubCompatible.
 Import ProcSyn.Core.
 Import unscoped.UnscopedNotations.
  
-
-
- (*  --- a bunch of tactics for replacement in conga and lt hypotheses  ---  *)
-Ltac subinallleft_lt  :=
- try match goal with
-| [H: lt ?P ?a ?P', Heq: ?ter=?P|- _] => symmetry in Heq; rewrite Heq in *; symmetry in Heq
-end .
-
-  
-Ltac subinallright_lt  :=
- try match goal with
-| [H: lt ?P ?a ?P', Heq: ?ter=?P'|- _] => symmetry in Heq; rewrite Heq in *; symmetry in Heq
-end .
-
-Ltac subinall_lt := subinallleft_lt; subinallright_lt. 
-
-Ltac subinallleft_conga  :=
- try match goal with
-| [H: conga ?P ?P', Heq: ?ter=?P|- _] => symmetry in Heq; rewrite Heq in *; symmetry in Heq
-end .
-
-
-Ltac subinallright_conga  :=
- try match goal with
-| [H: conga ?P ?P', Heq: ?ter=?P'|- _] => symmetry in Heq; rewrite Heq in *; symmetry in Heq
-end .
-
-Ltac subinall_conga := subinallleft_conga; subinallright_conga. 
-
-
-(*note that if terms are nested it won't work*)
-Ltac subinall := subinall_lt ; subinall_conga. 
-(*------------------------------*)
-
-
-
-Lemma conga_resp_sub: forall P Q sigma,
-  conga P Q -> conga (P [sigma]) (Q [sigma]).
-Proof.
-intros.
-inversion H.
-asimpl. eauto with picalc.
-asimpl. eauto with picalc.
-asimpl. eauto with picalc.
-Qed.
-
-Lemma cong_resp_sub: forall P Q sigma,
-  cong P Q -> cong (P [sigma]) (Q [sigma]).
-Proof.
-intros.
-generalize dependent sigma.
-induction H.
-intro.
-set ( D := conga_resp_sub P Q sigma H).
-eauto with picalc.
-eauto with picalc.
-eauto with picalc.
-eauto with picalc.
-asimpl. eauto with picalc.
-asimpl. eauto with picalc.
-asimpl. eauto with picalc.
-
-intro. 
-eapply Cg_ctxRcv.  
-eauto with picalc.
-Qed.
 
 
 
@@ -85,61 +20,39 @@ intros.
 inversion H.  (*caseAn on lt derivation*)
 (*======all the cases of Lt_send======*)  
 inversion H0 .
-subinall.   
-exfalso. inversion H0.
-subinall. 
-exfalso. inversion H0.
-subinall. 
-exfalso. inversion H0.
+subst. exfalso. inversion H0.
+subst. exfalso. inversion H0.
+subst. exfalso. inversion H0.
 (* ======all the cases of Lt_rcv======*)
 inversion H0.
-subinall.   
-exfalso. inversion H0.
-subinall. 
-exfalso. inversion H0.
-subinall. 
-exfalso. inversion H0.
+subst. exfalso. inversion H0.
+subst. exfalso. inversion H0.
+subst. exfalso. inversion H0.
 (*======all the cases parL======*)
 inversion H0.
 (*subcase com*)
 
 
-subinall.     
-inversion H2. (*destroy the AST*)
-econstructor . split. eapply Lt_parR.  
-symmetry in H8; rewrite H8 in *. eapply H1 .
-intuition .   
+subst.     
+inversion H5. (*destroy the AST*)
+eauto with picalc.
 (*subcase assoc*)  
 
-subinall.  
-inversion H2. (*destruct the AST*)
-(*rewrite H8 in H1.*)
-  (*caseAn on P1|Q1 ->a P'0*)
+subst.  
+inversion H5. (*destruct the AST*)
   subst.  
-  inversion H1.
-    
-  eexists. split.  
+  inversion H1. (*caseAn on P1|Q1 ->a P'0*)
   eauto with picalc.
-  intuition.
-
-  eexists. split.
   eauto with picalc.
-  intuition.
-
-  eexists. split.
   eauto with picalc.
-  intuition.
-
-  eexists. split.
   eauto with picalc.
-  intuition.
-
+  
 (*subcase neut*)
   
-  eexists. split.
-  subst.
+  eexists. split. 
+  subst. 
   inversion H5.
-  subst.
+  subst. 
   apply H1.
   subst. inversion H5.
   intuition.
@@ -148,24 +61,23 @@ inversion H2. (*destruct the AST*)
 inversion H0.
 (*subcase com*)
 
-eexists. split.
-subst.
-inversion H5.
+eexists. split. 
+subst. 
+inversion H5. 
 subst.
 eauto with picalc.
 subst. inversion H5. 
 intuition.
 
 (*subcase assoc*)
-(*subinall.*)  
-
+ 
 subst.
 
 (* caseAn on conga*)
 inversion H0.
  
 eexists. split.
-subst.
+subst. 
 eapply Lt_parL.
 eapply H1.
 subst.
@@ -369,7 +281,7 @@ generalize dependent Q'.
 generalize dependent a.
 induction H.
 
-(*case conga*)
+(*======case conga======*)
 intros. firstorder.
 assert (exists Q0, lt Q a Q0 /\ conga P' Q0).
 eapply Lconga_resp_lt.
@@ -382,12 +294,12 @@ eapply Rconga_resp_lt.
 eauto with picalc. auto.
 firstorder.
 eauto with picalc.
-(*case refl*)
+(*======case refl======*)
 
 firstorder.  
 eauto with picalc. 
 eauto with picalc.
-(*case sym*)
+(*======case sym======*)
 
 firstorder. 
 set (IHdestr := IHcong a P' P'). 
@@ -398,7 +310,7 @@ set (IHdestr := IHcong a Q' Q').
 firstorder .
 eauto with picalc.
 
-(*case trans*)
+(*======case trans======*)
 firstorder.
  
 set (D1:= IHcong1 a P' P').  destruct D1. 
@@ -410,39 +322,39 @@ firstorder.  eauto with picalc.
 set (D1:= IHcong2 a Q' P'). destruct D1.
 firstorder.
 set (D2 := IHcong1 a x P'). firstorder. eauto with picalc. 
-(*case parL*)
+(*======case parL======*)
 firstorder.   
 inversion H0. (*caseAn on P|Q ->a  ...*)
 subst.
-set (D1 := IHcong a Q' P'1 ). 
+set (D := IHcong a Q' P'1 ). 
 firstorder. eauto with picalc. 
  
 eauto with picalc.
 
 subst.
-set (D1:= IHcong (Lsend x y) Q' P'1). 
+set (D:= IHcong (Lsend x y) Q' P'1). 
 firstorder. eauto with picalc.
 
 subst.
-set (D1 := IHcong (Lrcv x y) Q' P'1).
+set (D := IHcong (Lrcv x y) Q' P'1).
 firstorder. eauto with picalc.
 (**)
 inversion H0. (*caseAn on P'|Q ->a  ...*)
 subst.
-set (D1 := IHcong a  P'1 Q). 
+set (D := IHcong a  P'1 Q). 
 firstorder. eauto with picalc.
  
 eauto with picalc.
  
 subst.
-set (D1 := IHcong (Lsend x y) P'1 Q ). 
+set (D := IHcong (Lsend x y) P'1 Q ). 
 firstorder. eauto with picalc.
 
 subst.
-set (D1 := IHcong (Lrcv x y) P'1 Q ). 
+set (D := IHcong (Lrcv x y) P'1 Q ). 
 firstorder.
 eauto with picalc.
-(*case parR*)
+(*======case parR======*)
 firstorder.
 inversion H0. (*caseAn on P|Q ->a  ...*)
 
@@ -450,15 +362,15 @@ subst.
 eauto with picalc.
 
 subst.
-set (D1 := IHcong a Q Q'1 ). firstorder.
+set (D := IHcong a Q Q'1 ). firstorder.
 eauto with picalc.
 
 subst. 
-set (D1:= IHcong (Lrcv x y) P Q'1). firstorder.
+set (D:= IHcong (Lrcv x y) P Q'1). firstorder.
 eauto with picalc.
 
 subst. 
-set (D1 := IHcong (Lsend x y) P Q'1). firstorder.
+set (D := IHcong (Lsend x y) P Q'1). firstorder.
 eauto with picalc.
 (**)
 inversion H0. (*caseAn on P|Q' ->a  ...*)
@@ -466,18 +378,18 @@ inversion H0. (*caseAn on P|Q' ->a  ...*)
 eauto with picalc. 
 
 subst.
-set (D1:= IHcong a Q'1 P). firstorder.
+set (D:= IHcong a Q'1 P). firstorder.
 eauto with picalc.
  
 subst.
-set (D1:= IHcong (Lrcv x y) Q'1 P). firstorder.
+set (D:= IHcong (Lrcv x y) Q'1 P). firstorder.
 eauto with picalc.
 
 subst.
-set (D1:= IHcong (Lsend x y) Q'1 P). firstorder.
+set (D:= IHcong (Lsend x y) Q'1 P). firstorder.
 eauto with picalc.
 
-(*case send*)
+(*======case send======*)
 firstorder. 
 inversion H0.
 subst.
@@ -487,7 +399,7 @@ inversion H0.
 subst.
 eauto with picalc.
 
-(*case rcv*)
+(*======case rcv======*)
 firstorder.
 inversion H0.
 subst. 
