theories/Normal.v
@@ -1,0 +1,160 @@
+
+Require Import ProcSyn.
+Require Import Semantics.
+Require Import SubCompatible.
+Import unscoped.UnscopedNotations.
+Require Import CongLtLemma.
+
+ 
+Lemma red_normal: forall P Q ,
+  red P Q -> exists S x y R1 R2, 
+     cong P  (Par  (Par (Send x y R1) (Rcv x R2))    S)   /\
+     cong Q  (Par (Par R1 (R2 [y..])  )   S) .
+Proof.
+intros.
+induction H. 
+firstorder.
+repeat eexists.
+eauto with picalc.
+eauto with picalc.
+
+firstorder.
+repeat eexists.
+eauto with picalc.
+
+eauto with picalc.
+ 
+asimpl.
+eauto with picalc.
+econstructor .
+repeat eexists.
+eauto with picalc.
+eauto with picalc.
+Qed.
+
+
+
+
+Lemma ltsend_normal: forall Q Q' x y, 
+  lt Q (Lsend x y)  Q' -> exists R S,  
+    cong Q (Par (Send x y R) S) /\ 
+    cong Q'(Par R S).
+Proof.
+intros.
+generalize dependent Q'.
+induction Q.
+ 
+(*======Q Zero======*)
+firstorder.
+exfalso. inversion H.
+
+(*======Q Par======*)
+firstorder.
+inversion H. (*caseAn on Q1|Q2 ->! ....*)
+subst.
+set (D := IHQ1 P' H4).
+firstorder. 
+repeat eexists.
+eauto with picalc.
+eauto with picalc.
+
+subst.
+set (D:= IHQ2 Q'0).
+firstorder.
+    
+repeat eexists.  
+eapply Cg_trans.
+eapply Cg_trans.
+eapply Cg_ctxParR.
+eapply H0.
+econstructor.
+eapply Cga_parCom.
+econstructor.
+eapply Cga_parAssoc.
+
+eapply Cg_trans.
+eapply Cg_trans.
+eapply Cg_ctxParR.
+eapply H1.
+econstructor.
+eapply Cga_parCom.
+eauto with picalc .
+(*======Q Rcv======*)
+firstorder. 
+exfalso. inversion H.  
+(*======Q Send======*) 
+firstorder.  
+inversion H.
+subst.
+repeat eexists.
+eauto with picalc.
+eauto with picalc.
+Qed.
+
+
+ 
+Lemma ltrcv_normal: forall Q Q' x y,
+  lt Q (Lrcv x y) Q' ->  exists R S,
+    cong Q (Par (Rcv x R) S)  /\  
+    cong Q' (Par (R[y..]) S) .
+Proof.
+intros.
+generalize dependent Q'.
+induction Q.
+
+(*======Q Zero======*)
+firstorder.
+exfalso. inversion H.
+(*======Q Par======*)
+firstorder.
+inversion H.  (*caseAn on Q1|Q2 --->? *)
+subst.
+set (D:= IHQ1 P' H4).
+firstorder. 
+repeat eexists.
+eauto with picalc.
+eauto with picalc.
+ 
+subst.
+set (D:= IHQ2 Q'0 H4).
+firstorder.
+repeat eexists. 
+eapply Cg_trans.
+eapply Cg_trans.
+eapply Cg_ctxParR.
+eapply H0.
+econstructor. eapply Cga_parCom.
+econstructor. eapply Cga_parAssoc.
+
+eapply Cg_trans.  
+eapply Cg_trans.
+eapply Cg_ctxParR.
+eapply H1.
+econstructor. eapply Cga_parCom.
+econstructor. eapply Cga_parAssoc.
+
+(*======Q Rcv======*) 
+firstorder.
+inversion H.
+subst. 
+repeat eexists.
+eauto with picalc.
+eauto with picalc.
+(*======Q Send======*)
+firstorder.  
+exfalso. inversion H.
+Qed.
+
+
+
+
+
+
+
+
+
+
+
+
+
+
