theories/SemEquiv.v
@@ -1,0 +1,179 @@
+Require Import ProcSyn.
+Require Import Semantics.
+Require Import SubCompatible.
+Import unscoped.UnscopedNotations.
+Require Import CongLtLemma.
+Require Import Normal.
+
+
+
+
+Theorem lttau_impl_red: forall P Q,
+  lt P Ltau Q -> red P Q.
+Proof.
+intros. 
+generalize dependent Q.
+induction P.
+
+(*======P Zero======*)
+firstorder. 
+exfalso. inversion H.
+(*======P Par======*)
+firstorder.  
+inversion H. (*caseAn on P1|P2--->tau ...*)  
+
+eauto with picalc.
+
+subst.
+set (D:= IHP2 Q' H4).
+eauto with picalc.
+
+ 
+subst.
+set (rnl := ltrcv_normal P2 Q' x y H3).
+set (snl := ltsend_normal P1 P' x y H2).
+firstorder.
+(*the derivation tree*)
+eapply Red_struc.
+eapply Cg_trans.
+eapply Cg_trans.
+eapply Cg_trans.
+eapply Cg_trans.
+eapply Cg_trans.
+eapply Cg_ctxParL.
+eapply H0.
+eapply Cg_ctxParR.
+eapply H4.
+econstructor. eapply Cga_parAssoc.
+eapply Cg_ctxParR. 
+econstructor. eapply Cga_parCom.
+eapply Cg_sym. 
+econstructor. eapply Cga_parAssoc. 
+eapply Cg_ctxParL.  
+eapply Cg_sym.
+econstructor. eapply Cga_parAssoc.
+
+eapply Red_par.
+eapply Red_par.
+eapply Red_comm.
+
+eapply Cg_trans.
+eapply Cg_trans.
+eapply Cg_trans.
+eapply Cg_trans.
+eapply Cg_trans.
+eapply Cg_ctxParL.
+eapply H1.
+eapply Cg_ctxParR.
+eapply H5.
+econstructor. eapply Cga_parAssoc.
+eapply Cg_ctxParR.
+econstructor. eapply Cga_parCom.
+eapply Cg_sym.
+econstructor. eapply Cga_parAssoc.
+eapply Cg_ctxParL.
+eapply Cg_sym.
+econstructor. eapply Cga_parAssoc.
+ 
+(*the other one*)
+subst.
+set (snl := ltsend_normal P2 Q' x y H3).
+set (rnl := ltrcv_normal P1 P' x y H2).
+firstorder. 
+eapply Red_struc.
+
+eapply Cg_trans.
+eapply Cg_trans.
+eapply Cg_trans.
+eapply Cg_trans.
+eapply Cg_trans.
+eapply Cg_ctxParL.
+eapply H0.
+eapply Cg_ctxParR.
+eapply H4.
+econstructor. eapply Cga_parAssoc.
+eapply Cg_ctxParR.
+econstructor. eapply Cga_parCom.
+eapply Cg_sym.
+econstructor. eapply Cga_parAssoc.
+eapply Cg_ctxParL.
+eapply Cg_sym.
+econstructor. eapply Cga_parAssoc.
+  
+eapply Red_par.
+eapply Red_par.
+eapply Red_struc. 
+econstructor. eapply Cga_parCom.
+eapply Red_comm.
+eapply Cg_refl.
+
+eapply Cg_trans.
+eapply Cg_trans.
+eapply Cg_trans.
+eapply Cg_trans.
+eapply Cg_trans.
+eapply Cg_trans.
+eapply Cg_trans.
+eapply Cg_trans.
+
+eapply Cg_ctxParL.
+eapply H1.
+eapply Cg_ctxParR.
+eapply H5.
+econstructor. eapply Cga_parCom.
+econstructor. eapply Cga_parAssoc.
+
+eapply Cg_ctxParR.
+eapply Cg_sym.
+econstructor. eapply Cga_parAssoc.
+
+eapply Cg_ctxParR.
+eapply Cg_ctxParL.
+econstructor. eapply Cga_parCom.
+
+eapply Cg_sym.
+econstructor. eapply Cga_parAssoc.
+  
+eapply Cg_ctxParL.
+eapply Cg_sym.
+econstructor. eapply Cga_parAssoc.
+ 
+eapply Cg_refl.
+(*======case Q Rcv======*)
+firstorder.
+exfalso. inversion H.
+(*======case Q Send======*)
+firstorder.
+exfalso. inversion H.
+Qed.
+
+
+
+
+Theorem red_impl_lt: forall P Q, red P Q -> 
+  exists Q', lt P Ltau Q' /\ cong Q Q'.
+Proof.
+intros.
+set (lem:= red_normal P Q). 
+ 
+firstorder. 
+assert(
+lt
+(Par (Par (Send x0 x1 x2) (Rcv x0 x3)) x)
+Ltau
+(Par (Par x2 x3[x1..]) x)
+).
+apply Lt_parL.
+eapply Lt_commL.
+eapply Lt_send.
+eapply Lt_rcv.
+set (lem:= cong_resp_lt (Par (Par (Send x0 x1 x2) (Rcv x0 x3)) x) P (Par (Par x2 x3[x1..]) x) Q Ltau).
+eapply Cg_sym in H0.
+firstorder.
+eexists. split. 
+eauto with picalc .
+eapply Cg_trans.
+eauto with picalc .
+auto with picalc .
+Qed.
+
