theories/SubCompatible.v
@@ -1,0 +1,40 @@
+
+Require Import ProcSyn.
+Require Import Semantics.
+Import unscoped.UnscopedNotations.
+
+
+
+
+Lemma conga_resp_sub: forall P Q sigma,
+  conga P Q -> conga (P [sigma]) (Q [sigma]).
+Proof.
+intros.
+inversion H.
+asimpl. eauto with picalc.
+asimpl. eauto with picalc.
+asimpl. eauto with picalc.
+Qed.
+
+Lemma cong_resp_sub: forall P Q sigma,
+  cong P Q -> cong (P [sigma]) (Q [sigma]).
+Proof.
+intros.
+generalize dependent sigma.
+induction H.
+intro.
+set ( D := conga_resp_sub P Q sigma H).
+eauto with picalc.
+eauto with picalc.
+eauto with picalc.
+eauto with picalc.
+asimpl. eauto with picalc.
+asimpl. eauto with picalc.
+asimpl. eauto with picalc.
+
+intro. 
+eapply Cg_ctxRcv.  
+eauto with picalc.
+Qed.
+
+Hint Resolve cong_resp_sub: sublem.
